lean/STLC/Main.lean
@@ -1,4 +1,15 @@
 import STLC
+import Lean
 
-def main : IO Unit :=
+open IO
+
+def main: IO Unit := do
   IO.println s!"Hello, cats!"
+  let counter ← IO.mkRef 0
+  let val1 ← counter.get
+  IO.println s!"Initial value: {val1}"
+  counter.modify (· + 1)
+  let val2 ← counter.get
+  IO.println s!"Updated value: {val2}"
+
+#eval main
